src/x86/instrrules/callrel.v
@@ -7,21 +7,7 @@ Require Import x86proved.common_tactics (* for [not] and [goal_has_evar] *).
 Require Import x86proved.basicspectac (* for [specapply *] *).
 Require Import x86proved.chargetac (* for [finish_logic] *).
 
-Lemma CALLrel_rule (p q: DWORD) (tgt: JmpTgt) (w sp:DWORD) :
-  |-- interpJmpTgt tgt q (fun P p' =>
-      (
-         safe @ (EIP ~= p' ** P ** ESP~=sp-#4 ** sp-#4 :-> q) -->>
-         safe @ (EIP ~= p  ** P ** ESP~=sp    ** sp-#4 :-> w)
-    ) <@ (p -- q :-> CALLrel tgt)).
-Proof.
-  rewrite /interpJmpTgt/interpMemSpecSrc.
-  do_instrrule
-    ((try specintros => *; autorewrite with push_at);
-     apply: TRIPLE_safe => ?;
-     do !instrrule_triple_bazooka_step idtac).
-Qed.
-
-Lemma CALLrel_loopy_rule (p q: DWORD) (tgt: JmpTgt) (w sp:DWORD):
+Lemma CALLrel_rule (p q: DWORD) (tgt: JmpTgt) (w sp:DWORD):
   |-- interpJmpTgt tgt q (fun P p' =>
       (
       |> safe @ (EIP ~= p' ** P ** ESP~=sp-#4 ** sp-#4 :-> q) -->>
@@ -38,38 +24,23 @@ Qed.
 (** We make this rule an instance of the typeclass, and leave
     unfolding things like [specAtDstSrc] to the getter tactic
     [get_instrrule_of]. *)
-(*Global Instance: forall tgt : JmpTgt, instrrule (CALLrel tgt) := fun tgt p q => @CALLrel_loopy_rule p q tgt.*)
 Global Instance: forall tgt : JmpTgt, instrrule (CALLrel tgt) := fun tgt p q => @CALLrel_rule p q tgt.
 
 Section specapply_hint.
 Local Hint Unfold interpJmpTgt : specapply.
 
+Ltac myspecapply R := (specapply R; last try rewrite <- spec_later_weaken).
 Corollary CALLrel_R_rule (r:Reg) (p q: DWORD) :
-  |-- Forall (w sp: DWORD) p', (
-         safe @ (EIP ~= p' ** r~=p' ** ESP~=sp-#4 ** sp-#4 :-> q) -->>
-         safe@ (EIP ~= p  ** r~=p' ** ESP~=sp    ** sp-#4 :-> w)
-    ) <@ (p -- q :-> CALLrel r).
-Proof. specintros => *. specapply *; finish_logic_with sbazooka. Qed.
-
-Corollary CALLrel_R_loopy_rule (r:Reg) (p q: DWORD) :
   |-- Forall (w sp: DWORD) p', (
       |> safe @ (EIP ~= p' ** r~=p' ** ESP~=sp-#4 ** sp-#4 :-> q) -->>
          safe @ (EIP ~= p  ** r~=p' ** ESP~=sp    ** sp-#4 :-> w)
     ) <@ (p -- q :-> CALLrel r).
-Proof. specintros => *. specapply (@CALLrel_loopy_rule p q r); finish_logic_with sbazooka. 
-Qed.
+Proof. specintros => *. myspecapply (@CALLrel_rule p q r); finish_logic_with sbazooka. Qed.
 
 Corollary CALLrel_I_rule (rel: DWORD) (p q: DWORD) :
-  |-- Forall (w sp: DWORD), (
-         safe @ (EIP ~= addB q rel ** ESP~=sp-#4 ** sp-#4 :-> q) -->>
-         safe @ (EIP ~= p          ** ESP~=sp    ** sp-#4 :-> w)
-    ) <@ (p -- q :-> CALLrel rel).
-Proof. specintros => *. specapply *; finish_logic_with sbazooka. Qed.
-
-Corollary CALLrel_I_loopy_rule (rel: DWORD) (p q: DWORD) :
   |-- Forall (w sp: DWORD), (
       |> safe @ (EIP ~= addB q rel ** ESP~=sp-#4 ** sp-#4 :-> q) -->>
          safe @ (EIP ~= p          ** ESP~=sp    ** sp-#4 :-> w)
     ) <@ (p -- q :-> CALLrel rel).
-Proof. specintros => *. specapply (@CALLrel_loopy_rule p q rel); finish_logic_with sbazooka. Qed.
+Proof. specintros => *. specapply (@CALLrel_rule p q rel); finish_logic_with sbazooka. Qed.
 End specapply_hint.
