src/x86/instrrules/jccrel.v
@@ -6,27 +6,13 @@ Require Import x86proved.triple (* for [triple_apply] *).
 Require Import x86proved.spectac (* for [eforalls] *).
 Require Import x86proved.common_tactics (* for [f_equiv'] *).
 
-Lemma JCCrel_loopy_rule (rel: DWORD) cc cv (b:bool) (p q: DWORD) :
+Lemma JCCrel_rule (rel: DWORD) cc cv (b:bool) (p q: DWORD) :
   |-- (
       |> safe @ (EIP ~= (if b == cv then addB q rel else q) ** ConditionIs cc b) -->>
       safe @ (EIP ~= p ** ConditionIs cc b)
     ) <@ (p -- q :-> JCCrel cc cv rel).
 Proof.
   apply: TRIPLE_safeLater => R. autounfold with instrrules_eval.
-  triple_apply triple_letGetCondition.
-  case: (b == cv).
-  { instrrule_triple_bazooka using do [ progress sbazooka | apply: lorR1 ]. }
-  { instrrule_triple_bazooka using do [ progress sbazooka | apply: lorR2 ]. }
-Qed.
-
-(** We also have a version where neither is under a [|>] operator *)
-Lemma JCCrel_rule (rel: DWORD) cc cv (b:bool) (p q: DWORD) :
-  |-- (
-      safe @ (EIP ~= (if b == cv then addB q rel else q) ** ConditionIs cc b ) -->>
-      safe @ (EIP ~= p ** ConditionIs cc b)
-    ) <@ (p -- q :-> JCCrel cc cv rel).
-Proof.
-  apply: TRIPLE_safe => R. autounfold with instrrules_eval.
   triple_apply triple_letGetCondition.
   case: (b == cv).
   { instrrule_triple_bazooka using do [ progress sbazooka | apply: lorR1 ]. }
