src/x86/wrapalloc.v
@@ -5,7 +5,7 @@ Require Import Ssreflect.ssreflect Ssreflect.ssrbool Ssreflect.ssrnat Ssreflect.
 Require Import x86proved.x86.procstate x86proved.x86.procstatemonad x86proved.bitsrep x86proved.bitsops x86proved.bitsprops x86proved.bitsopsprops.
 Require Import x86proved.spred x86proved.septac x86proved.spec x86proved.spectac x86proved.x86.basic x86proved.x86.program.
 Require Import x86proved.x86.call x86proved.x86.instr x86proved.x86.instrsyntax x86proved.x86.instrrules x86proved.x86.instrcodec x86proved.reader x86proved.pointsto x86proved.cursor x86proved.x86.inlinealloc
-               x86proved.x86.listspec x86proved.x86.listimp x86proved.triple x86proved.x86.macros.
+               x86proved.x86.listspec x86proved.x86.listimp x86proved.triple x86proved.x86.macros x86proved.chargetac.
 
 Set Implicit Arguments.
 Unset Strict Implicit.
@@ -46,18 +46,12 @@ specapply inlineAlloc_correct; first by ssimpl.
 specsplit.
 
 (* failure case *)
-autorewrite with push_at.
 
 (* MOV EDI, 0 *)
-specapply MOV_RanyI_rule. rewrite /RegToVReg. 
-- by ssimpl.
-rewrite <- spec_reads_frame. apply: limplAdj. apply: landL2.
-autorewrite with push_at. cancel1. rewrite /natAsDWORD/RegToVReg. 
-ssimpl. by apply: lorR2.
+specapply MOV_RanyI_rule; first by ssimpl. 
+finish_logic_with sbazooka. apply: lorR2. by rewrite /natAsDWORD.
 
 (* success case *)
-autorewrite with push_at.
-
 (* SUB EDI, bytes *)
 specintros => pb.
 
@@ -67,19 +61,13 @@ assert (H:= subB_equiv_addB_negB (pb+#bytes) # bytes).
 rewrite E0 in H. simpl (snd _) in H. rewrite addB_negBn in H.
 rewrite H in E0.
 
-specapply SUB_RI_rule. sbazooka.
+specapply SUB_RI_rule; first by ssimpl. 
 
 (* JMP SUCCEED *)
-specapply JMP_I_rule.
-- by ssimpl.
+specapply JMP_I_rule; first by ssimpl.
+rewrite <- spec_later_weaken. 
 
 (* Final stuff *)
-rewrite E0.
-rewrite <-spec_reads_frame.
-apply: limplAdj. autorewrite with push_at.
-apply: landL2. cancel1.
-rewrite /OSZCP/stateIsAny. sbazooka. apply: lorR1.
-
-simpl snd.
-sbazooka.
+rewrite E0. simpl snd. 
+finish_logic_with sbazooka. apply: lorR1. sbazooka. 
 Qed.
